add bn_get_ith_bit

code/bignum/Hacl.Bignum.Lib.fst
@@ -21,34 +21,33 @@ module Loops = Lib.LoopCombinators
 ///
 
 inline_for_extraction noextract
-val bn_is_bit_set:
+val bn_get_ith_bit:
     len:size_t
   -> b:lbignum len
   -> i:size_t{v i / 64 < v len} ->
-  Stack bool
+  Stack uint64
   (requires fun h -> live h b)
   (ensures  fun h0 r h1 -> h0 == h1 /\
-    r == S.bn_is_bit_set (as_seq h0 b) (v i))
+    r == S.bn_get_ith_bit (as_seq h0 b) (v i))
 
-let bn_is_bit_set len input ind =
+let bn_get_ith_bit len input ind =
   let i = ind /. 64ul in
   let j = ind %. 64ul in
   let tmp = input.(i) in
-  let tmp = (tmp >>. j) &. u64 1 in
-  FStar.UInt64.(Lib.RawIntTypes.u64_to_UInt64 tmp =^ 1uL)
+  (tmp >>. j) &. u64 1
 
 
 inline_for_extraction noextract
-val bn_bit_set:
+val bn_set_ith_bit:
     len:size_t
   -> b:lbignum len
   -> i:size_t{v i / 64 < v len} ->
   Stack unit
   (requires fun h -> live h b)
   (ensures  fun h0 _ h1 -> modifies (loc b) h0 h1 /\
-    as_seq h1 b == S.bn_bit_set (as_seq h0 b) (v i))
+    as_seq h1 b == S.bn_set_ith_bit (as_seq h0 b) (v i))
 
-let bn_bit_set len input ind =
+let bn_set_ith_bit len input ind =
   let i = ind /. 64ul in
   let j = ind %. 64ul in
   input.(i) <- input.(i) |. (u64 1 <<. j)
